Prefix: xsd: <http://www.w3.org/2001/XMLSchema#>
Prefix: owl: <http://www.w3.org/2002/07/owl#>
Prefix: : <http://www.example.com/>
Prefix: xml: <http://www.w3.org/XML/1998/namespace>
Prefix: rdf: <http://www.w3.org/1999/02/22-rdf-syntax-ns#>
Prefix: dc: <http://purl.org/dc/elements/1.1/>
Prefix: www: <http://www.example.com/>
Prefix: rdfs: <http://www.w3.org/2000/01/rdf-schema#>



Ontology: <http://www.example.com/>


Annotations: 
    rdfs:comment "中医药领域本体示例。"@zh,
    rdfs:comment "An example of OWL ontology for Traditional Chinese Medicine domain."@en

AnnotationProperty: rdfs:seeAlso

    
AnnotationProperty: rdfs:isDefinedBy

    
AnnotationProperty: rdfs:label

    
AnnotationProperty: rdfs:comment

    
Datatype: rdf:PlainLiteral

    
ObjectProperty: functionally_related_to

    SubPropertyOf: 
        associated_with
    
    EquivalentTo: 
        功能上相关
    
    
ObjectProperty: …的测量值

    Annotations: 
        rdfs:label "measurement of"@en,
        rdfs:label "…的测量值"@zh,
        rdfs:comment "The dimension, quantity, or capacity determined by measuring."@en,
        rdfs:comment "被测量了的尺寸、数量、容量值"@zh
    
    SubPropertyOf: 
        概念上相关
    
    EquivalentTo: 
        measurement_of
    
    
ObjectProperty: degree_of

    SubPropertyOf: 
        conceptually_related_to
    
    EquivalentTo: 
        …的程度-等级
    
    
ObjectProperty: physically_related_to

    SubPropertyOf: 
        associated_with
    
    EquivalentTo: 
        物理上相关
    
    
ObjectProperty: …之中的焦点问题

    Annotations: 
        rdfs:comment "Is an issue in or a point of discussion, study, debate, or dispute."@en,
        rdfs:label "issue in"@en,
        rdfs:label "…之中的焦点问题"@zh,
        rdfs:comment "讨论、研究、争论、辩论中的要点、关键。"@zh
    
    SubPropertyOf: 
        概念上相关
    
    EquivalentTo: 
        issue_in
    
    
ObjectProperty: tributary_of

    SubPropertyOf: 
        physically_related_to
    
    EquivalentTo: 
        由…汇合
    
    
ObjectProperty: 空间上相关

    Annotations: 
        rdfs:label "空间上相关"@zh,
        rdfs:label "spatially related to"@en,
        rdfs:comment "空间区域上的相关。"@zh,
        rdfs:comment "Related by place or region."@en
    
    SubPropertyOf: 
        相关关系链
    
    EquivalentTo: 
        spatially_related_to
    
    
ObjectProperty: 发生于…情况下

    Annotations: 
        rdfs:comment "Takes place in or happens under given conditions, circumstances, or time periods, or in a given location or population. This includes appears in, transpires, comes about, is present in, and exists in."@en,
        rdfs:label "发生于…情况下"@zh,
        rdfs:comment "在给定的条件、环境、时期里或给定的位置、场所或人口下发生。包括出现于、发生、产生、出现、存在等"@zh,
        rdfs:label "occurs in"@en
    
    SubPropertyOf: 
        功能上相关
    
    EquivalentTo: 
        occurs_in
    
    
ObjectProperty: 君药

    Annotations: 
        rdfs:label "has king"@en,
        rdfs:label "君药"@zh
    
    SubPropertyOf: 
        包含中草药
    
    
ObjectProperty: 带来-造成

    Annotations: 
        rdfs:comment "作用或影响一个实体"@zh,
        rdfs:label "带来-造成"@zh,
        rdfs:comment "Acts on or influences an entity."@en,
        rdfs:label "brings about"@en
    
    SubPropertyOf: 
        功能上相关
    
    EquivalentTo: 
        brings_about
    
    
ObjectProperty: similar_concepts

    SubPropertyOf: 
        conceptually_related_to
    
    EquivalentTo: 
        与…类似概念
    
    
ObjectProperty: 实施

    Annotations: 
        rdfs:label "carries out"@en,
        rdfs:comment "Executes a function or performs a procedure or activity. This includes transacts, operates on, handles, and executes."@en,
        rdfs:label "实施"@zh,
        rdfs:comment "执行一项功能或完成一项手续或活动。包括处理，操作、运转，操纵、运用，实行、执行等。"@zh
    
    SubPropertyOf: 
        执行
    
    EquivalentTo: 
        carries_out
    
    
ObjectProperty: disrupts

    SubPropertyOf: 
        affects
    
    EquivalentTo: 
        干扰
    
    
ObjectProperty: 有药味

    Annotations: 
        rdfs:label "has herbal taste"@en,
        rdfs:label "具有药味"@zh
    
    SubPropertyOf: 
        相关关系链
    
    Domain: 
        中药
    
    Range: 
        四气五味
    
    
ObjectProperty: …的方法

    Annotations: 
        rdfs:label "…的方法"@zh,
        rdfs:comment "The manner and sequence of events in performing an act or procedure"@en,
        rdfs:comment "事件在执行或完成一个动作或过程中的方式或顺序。"@zh,
        rdfs:label "method of"@en
    
    SubPropertyOf: 
        概念上相关
    
    EquivalentTo: 
        method_of
    
    
ObjectProperty: produces

    SubPropertyOf: 
        brings_about
    
    EquivalentTo: 
        产生
    
    
ObjectProperty: isa

    EquivalentTo: 
        等级关系链
    
    
ObjectProperty: connected_to

    SubPropertyOf: 
        physically_related_to
    
    EquivalentTo: 
        与…相连
    
    
ObjectProperty: brings_about

    SubPropertyOf: 
        functionally_related_to
    
    EquivalentTo: 
        带来-造成
    
    
ObjectProperty: exhibits

    SubPropertyOf: 
        performs
    
    EquivalentTo: 
        展示
    
    
ObjectProperty: 等级关系链

    Annotations: 
        rdfs:label "isa"@en,
        rdfs:comment ""@en,
        rdfs:comment ""@zh,
        rdfs:label "等级关系链"@en,
        rdfs:label "等级关系链"@zh
    
    EquivalentTo: 
        isa
    
    
ObjectProperty: 证实

    Annotations: 
        rdfs:comment "为一个实体或过程在某一时间的存在提供证据。"@zh,
        rdfs:label "indicates"@en,
        rdfs:comment "Gives evidence for the presence at some time of an entity or process."@en,
        rdfs:label "证实"@zh
    
    SubPropertyOf: 
        功能上相关
    
    EquivalentTo: 
        indicates
    
    
ObjectProperty: 影响

    Annotations: 
        rdfs:comment "改变或影响现有的条件、状态、情形、实体产生一种直接的效果。包括起作用，改变，影响，预先安排，刺激、促进，管理、控制、调节，压下，阻止，提高、增强，起作用、有助于、促成，引导、致使，更改、修改等。"@zh,
        rdfs:label "affects"@en,
        rdfs:comment "Produces a direct effect on. Implied here is the altering or influencing of an existing condition, state, situation, or entity. This includes has a role in, alters, influences, predisposes, catalyzes, stimulates, regulates, depresses, impedes, enhances, contributes to, leads to, and modifies."@en,
        rdfs:label "影响"@zh
    
    SubPropertyOf: 
        功能上相关
    
    EquivalentTo: 
        affects
    
    
ObjectProperty: 时间上相关

    Annotations: 
        rdfs:label "时间上相关"@zh,
        rdfs:label "temporally related to"@en,
        rdfs:comment "Related in time by preceding, co-occuring with, or following."@en,
        rdfs:comment "时间上的提前、同时、随后相关"@zh
    
    SubPropertyOf: 
        相关关系链
    
    EquivalentTo: 
        temporally_related_to
    
    
ObjectProperty: 与…相表里

    Annotations: 
        rdfs:label "inter exterior and interior with"@en,
        rdfs:comment ""@en,
        rdfs:comment "脏腑以及经络之间的阴阳表里关系，反映的是脏腑经络功能上的相互影响。"@zh,
        rdfs:label "与…相表里"@zh
    
    SubPropertyOf: 
        影响
    
    EquivalentTo: 
        inter_exterior_and_interior_with
    
    
ObjectProperty: …的评价

    Annotations: 
        rdfs:comment "Judgment of the value or degree of some attribute or process."@en,
        rdfs:comment "判断某种属性或过程的价值或程度。"@zh,
        rdfs:label "evaluation of"@en,
        rdfs:label "…的评价"@zh
    
    SubPropertyOf: 
        概念上相关
    
    EquivalentTo: 
        evaluation_of
    
    
ObjectProperty: 管理

    Annotations: 
        rdfs:comment "管理，有助于照顾个体或由个体组成的团体"@zh,
        rdfs:comment "Administers, or contributes to the care of an individual or group of individuals."@en,
        rdfs:label "管理"@zh,
        rdfs:label "manages"@en
    
    SubPropertyOf: 
        影响
    
    EquivalentTo: 
        manages
    
    
ObjectProperty: 概念上相关

    Annotations: 
        rdfs:label "概念上相关"@zh,
        rdfs:comment "Related by some abstract concept, thought, or idea."@en,
        rdfs:comment "被某些理论性的概念、思想和想法相关。"@zh,
        rdfs:label "conceptually related to"@en
    
    SubPropertyOf: 
        相关关系链
    
    EquivalentTo: 
        conceptually_related_to
    
    
ObjectProperty: …成份

    Annotations: 
        rdfs:comment "组成成分或构成成分。指一个部分的要素、成分。"@zh,
        rdfs:comment "Is a component of, as in a constituent of a preparation."@en,
        rdfs:label "…成份"@zh,
        rdfs:label "ingredient of"@en
    
    SubPropertyOf: 
        物理上相关
    
    EquivalentTo: 
        ingredient_of
    
    
ObjectProperty: 由…组成

    Annotations: 
        rdfs:comment "一个整体的结构上的组成部分或者某种材料或物质的构成部分。包括由…组成，由…构成，由…形成等。"@zh,
        rdfs:label "consists of"@en,
        rdfs:comment "Is structurally made up of in whole or in part of some material or matter. This includes composed of, made of, and formed of."@en,
        rdfs:label "由…组成"@zh
    
    SubPropertyOf: 
        物理上相关
    
    EquivalentTo: 
        consists_of
    
    
ObjectProperty: 使药

    Annotations: 
        rdfs:label "使药"@zh,
        rdfs:label "has messenger"@en
    
    SubPropertyOf: 
        包含中草药
    
    
ObjectProperty: temporally_related_to

    SubPropertyOf: 
        associated_with
    
    EquivalentTo: 
        时间上相关
    
    
ObjectProperty: interconnects

    SubPropertyOf: 
        physically_related_to
    
    EquivalentTo: 
        使…相互联系
    
    
ObjectProperty: 执行

    Annotations: 
        rdfs:label "执行"@zh,
        rdfs:comment "执行、实行；完成、实现：达到一种行为状态。"@zh,
        rdfs:comment "Executes, accomplishes, or achieves an activity."@en,
        rdfs:label "performs"@en
    
    SubPropertyOf: 
        功能上相关
    
    EquivalentTo: 
        performs
    
    
ObjectProperty: prevents

    SubPropertyOf: 
        affects
    
    EquivalentTo: 
        预防
    
    
ObjectProperty: …的进程

    Annotations: 
        rdfs:label "…的进程"@zh,
        rdfs:comment "行为，功能或状态？"@zh,
        rdfs:comment "Action, function, or state of."@en,
        rdfs:label "process of"@en
    
    SubPropertyOf: 
        发生于…情况下
    
    EquivalentTo: 
        process_of
    
    
ObjectProperty: complicates

    SubPropertyOf: 
        affects
    
    EquivalentTo: 
        并发
    
    
ObjectProperty: causes

    SubPropertyOf: 
        brings_about
    
    EquivalentTo: 
        引起
    
    
ObjectProperty: conceptually_related_to

    SubPropertyOf: 
        associated_with
    
    EquivalentTo: 
        概念上相关
    
    
ObjectProperty: derivative_of

    SubPropertyOf: 
        conceptually_related_to
    
    EquivalentTo: 
        衍生的
    
    
ObjectProperty: location_of

    SubPropertyOf: 
        spatially_related_to
    
    EquivalentTo: 
        位于…
    
    
ObjectProperty: 由…汇合

    Annotations: 
        rdfs:label "tributary of"@en,
        rdfs:comment "合并、并入。例如，血管的汇合。"@zh,
        rdfs:comment "Merges with. For example, the confluence of veins."@en,
        rdfs:label "由…汇合"@zh
    
    SubPropertyOf: 
        物理上相关
    
    EquivalentTo: 
        tributary_of
    
    
ObjectProperty: process_of

    SubPropertyOf: 
        occurs_in
    
    EquivalentTo: 
        …的进程
    
    
ObjectProperty: result_of

    SubPropertyOf: 
        functionally_related_to
    
    EquivalentTo: 
        …的结果-效果
    
    
ObjectProperty: measurement_of

    SubPropertyOf: 
        conceptually_related_to
    
    EquivalentTo: 
        …的测量值
    
    
ObjectProperty: method_of

    SubPropertyOf: 
        conceptually_related_to
    
    EquivalentTo: 
        …的方法
    
    
ObjectProperty: owl:topObjectProperty

    
ObjectProperty: 相关关系链

    Annotations: 
        rdfs:comment "有重要的或显著的关系"@zh,
        rdfs:label "associated with"@en,
        rdfs:comment "has a significant or salient relationship to"@en,
        rdfs:label "相关关系链"@zh
    
    EquivalentTo: 
        associated_with
    
    Characteristics: 
        Symmetric
    
    Domain: 
        临床状况
    
    Range: 
        临床状况
    
    
ObjectProperty: occurs_in

    SubPropertyOf: 
        functionally_related_to
    
    EquivalentTo: 
        发生于…情况下
    
    
ObjectProperty: …的部分

    Annotations: 
        rdfs:comment "Composes, with one or more other physical units, some larger whole. This includes component of, division of, portion of, fragment of, section of, and layer of."@en,
        rdfs:label "…的部分"@zh,
        rdfs:comment "有一个或更多个物理单位组成、构成某些较大的整体；包括…的成分，…的部分，…的片段，…的部件，…的层等。"@zh,
        rdfs:label "part of"@en
    
    SubPropertyOf: 
        物理上相关
    
    EquivalentTo: 
        part_of
    
    
ObjectProperty: 先于…发生

    Annotations: 
        rdfs:comment "Occurs earlier in time. This includes antedates, comes before, is in advance of, predates, and is prior to."@en,
        rdfs:label "precedes"@en,
        rdfs:comment "提前发生。包括比实际提前的时间，在…之前发生，提前的，预先的，优先的"@zh,
        rdfs:label "先于…发生"@zh
    
    SubPropertyOf: 
        时间上相关
    
    EquivalentTo: 
        precedes
    
    
ObjectProperty: surrounds

    SubPropertyOf: 
        spatially_related_to
    
    EquivalentTo: 
        包围-周围
    
    
ObjectProperty: ingredient_of

    SubPropertyOf: 
        physically_related_to
    
    EquivalentTo: 
        …成份
    
    
ObjectProperty: issue_in

    SubPropertyOf: 
        conceptually_related_to
    
    EquivalentTo: 
        …之中的焦点问题
    
    
ObjectProperty: 传递性下位概念

    Annotations: 
        rdfs:label "narrowerTransitive"@en,
        rdfs:label "传递性下位概念"@zh
    
    SubPropertyOf: 
        等级关系链
    
    
ObjectProperty: manages

    SubPropertyOf: 
        affects
    
    EquivalentTo: 
        管理
    
    
ObjectProperty: 并发

    Annotations: 
        rdfs:comment "Causes to become more severe or complex or results in adverse effects."@en,
        rdfs:comment "引起变得更严重或更复杂或产生一种不利的结果。"@zh,
        rdfs:label "complicates"@en,
        rdfs:label "并发"@zh
    
    SubPropertyOf: 
        影响
    
    EquivalentTo: 
        complicates
    
    
ObjectProperty: 治疗

    Annotations: 
        rdfs:comment "Applies a remedy with the object of effecting a cure or managing a condition."@en,
        rdfs:label "treats"@en,
        rdfs:comment "提供一种治愈或改善症状的疗法"@zh,
        rdfs:label "治疗"@zh
    
    SubPropertyOf: 
        相关关系链,
        影响
    
    EquivalentTo: 
        treats
    
    Domain: 
        治法
         or 药用物质
    
    Range: 
        临床状况
    
    
ObjectProperty: 位于…

    Annotations: 
        rdfs:comment "The position, site, or region of an entity or the site of a process."@en,
        rdfs:comment "位置、场所，一个实体的位置或一个过程的场所。"@zh,
        rdfs:label "location of"@en,
        rdfs:label "位于…"@zh
    
    SubPropertyOf: 
        空间上相关
    
    EquivalentTo: 
        location_of
    
    
ObjectProperty: 生

    Annotations: 
        rdfs:label "engenders"@en,
        rdfs:label "生"@zh
    
    SubPropertyOf: 
        影响
    
    
ObjectProperty: 产生

    Annotations: 
        rdfs:comment "提出、带来、产生、创造。包括出产、生长、生产，分泌，放射、发出，用生物学的方法合成，产生，释放，放出，创造、引起、造成等。"@zh,
        rdfs:label "produces"@en,
        rdfs:comment "Brings forth, generates or creates. This includes yields, secretes, emits, biosynthesizes, generates, releases, discharges, and creates."@en,
        rdfs:label "产生"@zh
    
    SubPropertyOf: 
        带来-造成
    
    EquivalentTo: 
        produces
    
    
ObjectProperty: …的概念部分

    Annotations: 
        rdfs:comment "Conceptually a portion, division, or component of some larger whole."@en,
        rdfs:comment "概念的一部分，或某个较大整体的组成成分。"@zh,
        rdfs:label "conceptual part of"@en,
        rdfs:label "…的概念部分"@zh
    
    SubPropertyOf: 
        概念上相关
    
    EquivalentTo: 
        conceptual_part_of
    
    
ObjectProperty: 展示

    Annotations: 
        rdfs:comment "表示、出示、证明等。"@zh,
        rdfs:label "展示"@zh,
        rdfs:comment "Shows or demonstrates."@en,
        rdfs:label "exhibits"@en
    
    SubPropertyOf: 
        执行
    
    EquivalentTo: 
        exhibits
    
    
ObjectProperty: 衍生的

    Annotations: 
        rdfs:label "derivative of"@en,
        rdfs:comment "化学上，一种物质与另一种物质在结构上相关，或者能够被其他的物质所产生。这仅仅指结构上的关联。不包括功能上的关联比如.…的代谢物，.…的产物，.…的类似物。"@zh,
        rdfs:comment "In chemistry, a substance structurally related to another or that can be made from the other substance. This is used only for structural relationships. This does not include functional relationships such as metabolite of, by product of, nor analog of."@en,
        rdfs:label "衍生的"@zh
    
    SubPropertyOf: 
        概念上相关
    
    EquivalentTo: 
        derivative_of
    
    
ObjectProperty: 引起

    Annotations: 
        rdfs:comment "Brings about a condition or an effect. Implied here is that an agent, such as for example, a pharmacologic substance or an organism, has brought about the effect. This includes induces, effects, evokes, and etiology."@en,
        rdfs:label "引起"@zh,
        rdfs:comment "引起一种状态或结果。这里所指的是一种原因，例如，一种药物或有机体产生的结果。包括引起，导致，唤起，病变的原因。"@zh,
        rdfs:label "causes"@en
    
    SubPropertyOf: 
        带来-造成
    
    EquivalentTo: 
        causes
    
    
ObjectProperty: 穿过

    Annotations: 
        rdfs:label "traverses"@en,
        rdfs:comment "Crosses or extends across another physical structure or area. This includes crosses over and crosses through."@en,
        rdfs:comment "穿过或者延伸越过另一个物理结构或区域。包括从其上跨过和从其中穿过。"@zh,
        rdfs:label "穿过"@zh
    
    SubPropertyOf: 
        空间上相关
    
    EquivalentTo: 
        traverses
    
    
ObjectProperty: 开处方

    Annotations: 
        rdfs:label "开处方"@zh,
        rdfs:label "prescribes"@en
    
    SubPropertyOf: 
        相关关系链
    
    Domain: 
        治法
    
    Range: 
        药用物质
    
    
ObjectProperty: part_of

    SubPropertyOf: 
        physically_related_to
    
    EquivalentTo: 
        …的部分
    
    
ObjectProperty: manifestation_of

    SubPropertyOf: 
        functionally_related_to
    
    EquivalentTo: 
        现象表达
    
    
ObjectProperty: 包含

    Annotations: 
        rdfs:comment "包含"@zh,
        rdfs:comment "Holds or is the receptacle for fluids or other substances. This includes is filled with, holds, and is occupied by."@en,
        rdfs:label "包含"@zh,
        rdfs:label "contains"@en,
        rdfs:comment "可容纳或者是一个贮藏液体或其他物质的容器。包括被…充满，可容纳，被…占用等。"@zh
    
    SubPropertyOf: 
        相关关系链,
        物理上相关
    
    EquivalentTo: 
        contains
    
    
ObjectProperty: assesses_effect_of

    SubPropertyOf: 
        analyzes
    
    EquivalentTo: 
        分析评估…的影响
    
    
ObjectProperty: 分析

    Annotations: 
        rdfs:label "分析"@zh,
        rdfs:comment "Studies or examines using established quantitative or qualitative methods."@en,
        rdfs:label "analyzes"@en,
        rdfs:comment "用确定的定量的或定型的方法研究或检查。"@zh
    
    SubPropertyOf: 
        概念上相关
    
    EquivalentTo: 
        analyzes
    
    
ObjectProperty: 包含中草药

    Annotations: 
        rdfs:label "contains herb"@en,
        rdfs:label "包含中草药"@zh
    
    SubPropertyOf: 
        包含
    
    Domain: 
        方剂
    
    Range: 
        中药
    
    
ObjectProperty: 分析评估…的影响

    Annotations: 
        rdfs:label "assesses effect of"@en,
        rdfs:comment "Analyzes the influence or consequences of the function or action of."@en,
        rdfs:comment "分析功能或行为的影响或结果。"@zh,
        rdfs:label "分析评估…的影响"@zh
    
    SubPropertyOf: 
        分析
    
    EquivalentTo: 
        assesses_effect_of
    
    
ObjectProperty: 干扰

    Annotations: 
        rdfs:label "disrupts"@en,
        rdfs:label "干扰"@zh,
        rdfs:comment "改变或影响一个已经存在的条件、状态或情形，产生一种消极的影响。"@zh,
        rdfs:comment "Alters or influences an already existing condition, state, or situation. Produces a negative effect on."@en
    
    SubPropertyOf: 
        影响
    
    EquivalentTo: 
        disrupts
    
    
ObjectProperty: 被使用

    SubPropertyOf: 
        功能上相关
    
    InverseOf: 
        使用
    
    
ObjectProperty: 与…相邻

    Annotations: 
        rdfs:comment "与另一个物理单位紧密地相连的，邻接的，没有其他的同样的结构介入其中。包括毗邻，邻接，邻近的，并列的，紧密联结的。"@zh,
        rdfs:label "adjacent to"@en,
        rdfs:comment "Close to, near or abutting another physical unit with no other structure of the same kind intervening. This includes adjoins, abuts, is contiguous to, is juxtaposed, and is close to."@en,
        rdfs:label "与…相邻"@zh
    
    SubPropertyOf: 
        空间上相关
    
    EquivalentTo: 
        adjacent_to
    
    
ObjectProperty: 测量

    Annotations: 
        rdfs:label "测量"@zh,
        rdfs:comment "确定或标记尺寸、数量、程度、容量等。"@zh,
        rdfs:comment "Ascertains or marks the dimensions, quantity, degree, or capacity of."@en,
        rdfs:label "measures"@en
    
    SubPropertyOf: 
        概念上相关
    
    EquivalentTo: 
        measures
    
    
ObjectProperty: treats

    SubPropertyOf: 
        affects
    
    EquivalentTo: 
        治疗
    
    
ObjectProperty: contains

    SubPropertyOf: 
        physically_related_to
    
    EquivalentTo: 
        包含
    
    
ObjectProperty: 包含化学物质

    Annotations: 
        rdfs:label "包含化学物质"@zh,
        rdfs:label "contains chemical"@en
    
    SubPropertyOf: 
        包含
    
    Domain: 
        中药
    
    Range: 
        化学物质
    
    
ObjectProperty: spatially_related_to

    SubPropertyOf: 
        associated_with
    
    EquivalentTo: 
        空间上相关
    
    
ObjectProperty: 与…相连

    Annotations: 
        rdfs:comment "Directly attached to another physical unit as tendons are connected to muscles. This includes attached to and anchored to."@en,
        rdfs:label "connected to"@en,
        rdfs:label "与…相连"@zh,
        rdfs:comment "直接地附着在另一个物理单元上，比如肌腱与肌肉相连。包括附着在…上，固定在…上。"@zh
    
    SubPropertyOf: 
        物理上相关
    
    EquivalentTo: 
        connected_to
    
    
ObjectProperty: …的发育阶段

    Annotations: 
        rdfs:comment "个体成熟过程中的早期阶段。"@zh,
        rdfs:label "developmental form of"@en,
        rdfs:label "…的发育阶段"@zh,
        rdfs:comment "An earlier stage in the individual maturation of."@en
    
    SubPropertyOf: 
        概念上相关
    
    EquivalentTo: 
        developmental_form_of
    
    
ObjectProperty: 的病位是

    Annotations: 
        rdfs:label "has location"@en,
        rdfs:label "的病位是"@zh
    
    SubPropertyOf: 
        相关关系链
    
    
ObjectProperty: indicates

    SubPropertyOf: 
        functionally_related_to
    
    EquivalentTo: 
        证实
    
    
ObjectProperty: 使…相互联系

    Annotations: 
        rdfs:comment "Serves to link or join together two or more other physical units. This includes joins, links, conjoins, articulates, separates, and bridges."@en,
        rdfs:label "interconnects"@en,
        rdfs:label "使…相互联系"@zh,
        rdfs:comment "使两个或多个物理单元连接或结合在一起。包括结合，连接，连结，用关节连接，分离？桥梁连接等。"@zh
    
    SubPropertyOf: 
        物理上相关
    
    EquivalentTo: 
        interconnects
    
    
ObjectProperty: meridian_tropism

    SubPropertyOf: 
        affects
    
    EquivalentTo: 
        归…经
    
    
ObjectProperty: property_of

    SubPropertyOf: 
        conceptually_related_to
    
    EquivalentTo: 
        …的特性
    
    
ObjectProperty: analyzes

    SubPropertyOf: 
        conceptually_related_to
    
    EquivalentTo: 
        分析
    
    
ObjectProperty: 功能上相关

    Annotations: 
        rdfs:label "功能上相关"@zh,
        rdfs:comment "Related by the carrying out of some function or activity."@en,
        rdfs:label "functionally related to"@en,
        rdfs:comment "由于某些功能或者活动而相关。"@zh
    
    SubPropertyOf: 
        相关关系链
    
    EquivalentTo: 
        functionally_related_to
    
    
ObjectProperty: uses

    SubPropertyOf: 
        functionally_related_to
    
    EquivalentTo: 
        使用
    
    
ObjectProperty: carries_out

    SubPropertyOf: 
        performs
    
    EquivalentTo: 
        实施
    
    
ObjectProperty: practices

    SubPropertyOf: 
        performs
    
    EquivalentTo: 
        练习
    
    
ObjectProperty: 与…相互作用

    Annotations: 
        rdfs:label "interacts with"@en,
        rdfs:comment "Acts, functions, or operates together with"@en,
        rdfs:label "与…相互作用"@zh,
        rdfs:comment "与…一起产生效果，起作用"@zh
    
    SubPropertyOf: 
        影响
    
    EquivalentTo: 
        interacts_with
    
    
ObjectProperty: 与…类似概念

    Annotations: 
        rdfs:comment ""@en,
        rdfs:label "similar concepts"@en,
        rdfs:comment ""@zh,
        rdfs:label "与…类似概念"@zh
    
    SubPropertyOf: 
        概念上相关
    
    EquivalentTo: 
        similar_concepts
    
    
ObjectProperty: co-occurs_with

    SubPropertyOf: 
        temporally_related_to
    
    EquivalentTo: 
        与…同时发生
    
    
ObjectProperty: consists_of

    SubPropertyOf: 
        physically_related_to
    
    EquivalentTo: 
        由…组成
    
    
ObjectProperty: interacts_with

    SubPropertyOf: 
        affects
    
    EquivalentTo: 
        与…相互作用
    
    
ObjectProperty: inter_exterior_and_interior_with

    SubPropertyOf: 
        affects
    
    EquivalentTo: 
        与…相表里
    
    
ObjectProperty: affects

    SubPropertyOf: 
        functionally_related_to
    
    EquivalentTo: 
        影响
    
    
ObjectProperty: 练习

    Annotations: 
        rdfs:label "练习"@zh,
        rdfs:label "practices"@en,
        rdfs:comment "习惯地通常地进行、实行。"@zh,
        rdfs:comment "Performs habitually or customarily."@en
    
    SubPropertyOf: 
        执行
    
    EquivalentTo: 
        practices
    
    
ObjectProperty: traverses

    SubPropertyOf: 
        spatially_related_to
    
    EquivalentTo: 
        穿过
    
    
ObjectProperty: 归…经

    Annotations: 
        rdfs:comment ""@en,
        rdfs:label "归…经"@zh,
        rdfs:comment "是药物对机体某部分的选择性作用。归是作用的归属，经是脏腑经络的概称"@zh,
        rdfs:label "meridian tropism"@en
    
    SubPropertyOf: 
        影响
    
    EquivalentTo: 
        meridian_tropism
    
    
ObjectProperty: 分支

    Annotations: 
        rdfs:comment "Arises from the division of. For example, the arborization of arteries."@en,
        rdfs:label "分支"@zh,
        rdfs:comment "出现于分开的部分。例如，动脉的分支。"@zh,
        rdfs:label "branch of"@en
    
    SubPropertyOf: 
        物理上相关
    
    EquivalentTo: 
        branch_of
    
    
ObjectProperty: 传递性上位概念

    Annotations: 
        rdfs:label "broaderTransitive"@en,
        rdfs:label "传递性上位概念"@zh
    
    SubPropertyOf: 
        等级关系链
    
    
ObjectProperty: measures

    SubPropertyOf: 
        conceptually_related_to
    
    EquivalentTo: 
        测量
    
    
ObjectProperty: 滋养

    Annotations: 
        rdfs:label "nourishes"@en,
        rdfs:label "滋养"@zh
    
    SubPropertyOf: 
        生
    
    
ObjectProperty: 诊断

    Annotations: 
        rdfs:comment "区别或鉴别特性或特征。"@zh,
        rdfs:label "diagnoses"@en,
        rdfs:comment "Distinguishes or identifies the nature or characteristics of."@en,
        rdfs:label "诊断"@zh
    
    SubPropertyOf: 
        概念上相关
    
    EquivalentTo: 
        diagnoses
    
    
ObjectProperty: 预防

    Annotations: 
        rdfs:label "预防"@zh,
        rdfs:comment "Stops, hinders or eliminates an action or condition."@en,
        rdfs:comment "停止、阻碍或消除一种行为或状态。"@zh,
        rdfs:label "prevents"@en
    
    SubPropertyOf: 
        影响
    
    EquivalentTo: 
        prevents
    
    
ObjectProperty: …的特性

    Annotations: 
        rdfs:comment "…的特征、特性，.…的品质、性质。"@zh,
        rdfs:comment "Characteristic of, or quality of."@en,
        rdfs:label "property of"@en,
        rdfs:label "…的特性"@zh
    
    SubPropertyOf: 
        概念上相关
    
    EquivalentTo: 
        property_of
    
    
ObjectProperty: 与…同时发生

    Annotations: 
        rdfs:comment "在同一时间一起或者共同地、连带地发生。包括同时发生的，并发的，同时期发生的，伴发的，共存的，伴随产生的等。"@zh,
        rdfs:label "co-occurs with"@en,
        rdfs:comment "Occurs at the same time as, together with, or jointly. This includes is co-incident with, is concurrent with, is contemporaneous with, accompanies, coexists with, and is concomitant with."@en,
        rdfs:label "与…同时发生"@zh
    
    SubPropertyOf: 
        时间上相关
    
    EquivalentTo: 
        co-occurs_with
    
    
ObjectProperty: 现象表达

    Annotations: 
        rdfs:label "manifestation of"@en,
        rdfs:label "现象表达"@zh,
        rdfs:comment "能直接地可见的或者能具体地明显地被表示的现象的部分，能显示潜在的过程的现象部分。包括表达，表明，展示，显示等。"@zh,
        rdfs:comment "That part of a phenomenon which is directly observable or concretely or visibly expressed, or which gives evidence to the underlying process. This includes expression of, display of, and exhibition of."@en
    
    SubPropertyOf: 
        功能上相关
    
    EquivalentTo: 
        manifestation_of
    
    
ObjectProperty: evaluation_of

    SubPropertyOf: 
        conceptually_related_to
    
    EquivalentTo: 
        …的评价
    
    
ObjectProperty: 物理上相关

    Annotations: 
        rdfs:comment "Related by virtue of some physical attribute or characteristic."@en,
        rdfs:label "physically related to"@en,
        rdfs:comment "由于某些物理的属性或特征而相关"@zh,
        rdfs:label "物理上相关"@zh
    
    SubPropertyOf: 
        相关关系链
    
    EquivalentTo: 
        physically_related_to
    
    
ObjectProperty: 佐药

    Annotations: 
        rdfs:label "佐药"@zh,
        rdfs:label "has subordinate"@en
    
    SubPropertyOf: 
        包含中草药
    
    
ObjectProperty: associated_with

    EquivalentTo: 
        相关关系链
    
    
ObjectProperty: 包围-周围

    Annotations: 
        rdfs:comment "确立分界线，定义另一个物理结构的界限。包括界限，范围，界线，围住、在…周围化线。"@zh,
        rdfs:comment "Establishes the boundaries for, or defines the limits of another physical structure. This includes limits, bounds, confines, encloses, and circumscribes."@en,
        rdfs:label "surrounds"@en,
        rdfs:label "包围-周围"@zh
    
    SubPropertyOf: 
        空间上相关
    
    EquivalentTo: 
        surrounds
    
    
ObjectProperty: developmental_form_of

    SubPropertyOf: 
        conceptually_related_to
    
    EquivalentTo: 
        …的发育阶段
    
    
ObjectProperty: …的程度-等级

    Annotations: 
        rdfs:label "…的程度-等级"@zh,
        rdfs:comment "The relative intensity of a process or the relative intensity or amount of a quality or attribute."@en,
        rdfs:comment "一个过程相对的强度，一种属性或性质的相对强度或数量。"@zh,
        rdfs:label "degree of"@en
    
    SubPropertyOf: 
        概念上相关
    
    EquivalentTo: 
        degree_of
    
    
ObjectProperty: precedes

    SubPropertyOf: 
        temporally_related_to
    
    EquivalentTo: 
        先于…发生
    
    
ObjectProperty: branch_of

    SubPropertyOf: 
        physically_related_to
    
    EquivalentTo: 
        分支
    
    
ObjectProperty: conceptual_part_of

    SubPropertyOf: 
        conceptually_related_to
    
    EquivalentTo: 
        …的概念部分
    
    
ObjectProperty: …的结果-效果

    Annotations: 
        rdfs:comment "The condition, product, or state occurring as a consequence, effect, or conclusion of an activity or process. This includes product of, effect of, sequel of, outcome of, culmination of, and completion of."@en,
        rdfs:comment "状态、情况、结果作为一个结果、效果或一个活动或过程的结论结局而发生。包括…的结果，…的效果，…的结局，…的成果，…的顶点，…的完成。"@zh,
        rdfs:label "…的结果-效果"@zh,
        rdfs:label "result of"@en
    
    SubPropertyOf: 
        功能上相关
    
    EquivalentTo: 
        result_of
    
    
ObjectProperty: 臣药

    Annotations: 
        rdfs:label "has minister"@en,
        rdfs:label "臣药"@zh
    
    SubPropertyOf: 
        包含中草药
    
    
ObjectProperty: adjacent_to

    SubPropertyOf: 
        spatially_related_to
    
    EquivalentTo: 
        与…相邻
    
    
ObjectProperty: performs

    SubPropertyOf: 
        functionally_related_to
    
    EquivalentTo: 
        执行
    
    
ObjectProperty: diagnoses

    SubPropertyOf: 
        conceptually_related_to
    
    EquivalentTo: 
        诊断
    
    
ObjectProperty: 使用

    Annotations: 
        rdfs:label "使用"@zh,
        rdfs:comment "Employs in the carrying out of some activity. This includes applies, utilizes, employs, and avails."@en,
        rdfs:label "uses"@en,
        rdfs:comment "在某些正在进行的活动中使用。包括应用、适用、利用、使用等。"@zh
    
    SubPropertyOf: 
        功能上相关
    
    EquivalentTo: 
        uses
    
    InverseOf: 
        被使用
    
    
Class: 植物

    Annotations: 
        rdfs:label "Plant"@en,
        rdfs:label "植物"@zh
    
    SubClassOf: 
        有机体
    
    
Class: 五行

    Annotations: 
        rdfs:label "五行"@zh,
        rdfs:label "five phases"@en
    
    SubClassOf: 
        五行理论
    
    
Class: 物理对象

    Annotations: 
        rdfs:comment "An object perceptible to the sense of vision or touch. (UMLS)"@zh,
        rdfs:label "物理对象"@zh,
        rdfs:label "Physical object"@en
    
    SubClassOf: 
        实体
    
    
Class: 化学物质

    Annotations: 
        rdfs:label "Chemical"@en,
        rdfs:label "化学物质"@zh,
        rdfs:comment "具有特定的分子组成，并作为化学过程的参与者或产物的物质."@zh,
        rdfs:comment "A substance with a distinct molecular composition that is produced by or used in a chemical process."@en
    
    SubClassOf: 
        物质
    
    
Class: 药用动物植物矿物

    Annotations: 
        rdfs:label "Medicinal animal plant and mineral"@en,
        rdfs:comment "Generally refers to all animals, plants and minerals that can be used as drugs."@en,
        rdfs:label "药用动物、植物和矿物质"@zh
    
    SubClassOf: 
        物理对象
    
    
Class: 事件

    Annotations: 
        rdfs:label "A broad type for grouping activities, processes and states.(UMLS)"@zh,
        rdfs:label "事件"@zh,
        rdfs:label "Event"@en
    
    SubClassOf: 
        owl:Thing
    
    
Class: 六腑

    SubClassOf: 
        腑
    
    
Class: 临床状况

    Annotations: 
        rdfs:label "clinical finding"@en,
        rdfs:label "临床发现"@zh
    
    SubClassOf: 
        病因病机疾病
    
    
Class: 精

    Annotations: 
        rdfs:label "精"@zh,
        rdfs:label "Essence"@en,
        rdfs:comment "Essence means two things: (1) the fundamental substance that builds up the physical structure and maintains body function; (2) reproductive essence stored in the kidney."@en
    
    SubClassOf: 
        人体基本物质
    
    
Class: 五味

    Annotations: 
        rdfs:label "五味"@zh,
        rdfs:label "five herbal taste"@en
    
    EquivalentTo: 
        {咸 , 甜 , 苦 , 辛 , 酸}
    
    SubClassOf: 
        四气五味
    
    
Class: 团体

    Annotations: 
        rdfs:label "Organization"@en,
        rdfs:label "团体"@zh
    
    SubClassOf: 
        概念实体
    
    
Class: 中医人体基础

    Annotations: 
        rdfs:label "Basic material in the human body in Chinese medicine"@en,
        rdfs:comment "In Chinese medicine, the basic elements, constituents, or substances of which the human body is composed or can be made according to TCM theory."@en,
        rdfs:label "中医人体基础"@zh
    
    SubClassOf: 
        物理对象
    
    
Class: 草药

    Annotations: 
        rdfs:label "草药"@zh,
        rdfs:comment "Herbal medicines include herbs, herbal materials, herbal preparations and finished herbal products, that contain as active ingredients parts of plants, or other plant materials, or combinations thereof."@en,
        rdfs:comment "草药包括含有植物、植物原料或其组合等活性成分的药草、药草原料、药草制剂及药草成本."@zh,
        rdfs:label "Herb"@en
    
    SubClassOf: 
        药用物质
    
    
Class: 药用动物

    Annotations: 
        rdfs:comment "Generally refers to those animals that have health function or can be used to prevent and treat the disease."@zh,
        rdfs:comment "Medicinal animal"@en,
        rdfs:comment "药用动物"@zh
    
    SubClassOf: 
        药用动物植物矿物
    
    
Class: 症状体征

    Annotations: 
        rdfs:label "症状体征"@zh,
        rdfs:comment "A (bodily or mental) phenomenon, circumstance, or change of condition arising from and accompanying a disease or other pathological condition, and constituting an indication or evidence of it; a characteristic sign of a particular disease. Especially, in modern use, a subjective indication, perceptible to the patient."@en,
        rdfs:label "Symptom & sign"@en
    
    SubClassOf: 
        病因病机疾病
    
    
Class: 中医理论

    Annotations: 
        rdfs:label "Traditional Chinese medicine theory"@en,
        rdfs:comment "In Chinese medicine, a system of ideas formed from Chinese medical philosophy in combination with practical experiences on medicine, such as yin-yang theory, visceral manifestation theory, meridian and collateral theory, essential qi theory, and five-phase theory."@en,
        rdfs:label "中医理论"@zh
    
    SubClassOf: 
        概念实体
    
    
Class: 实体

    Annotations: 
        rdfs:comment "A broad type for grouping physical and conceptual entities."@zh,
        rdfs:label "Entity"@en,
        rdfs:label "实体"@zh
    
    
Class: 功能性人体系统

    Annotations: 
        rdfs:label "功能性人体系统"@zh,
        rdfs:label "Functional body system"@en
    
    SubClassOf: 
        中医人体基础
    
    
Class: 气

    Annotations: 
        rdfs:label "Qi"@en,
        rdfs:comment "The basic element that constitutes the cosmos and, through its movements, changes and transformations, produces everything in the world, including the human body and life activities. In the field of medicine, qi refers both to the refined nutritive substance that flows within the human body as well as to its functional activities."@en,
        rdfs:label "气"@zh
    
    SubClassOf: 
        人体基本物质
    
    
Class: 药性

    Annotations: 
        rdfs:label "Nature of Chinese medicinals"@en,
        rdfs:label "药性"@zh,
        rdfs:comment "The basic properties of a medicinal mainly includes four qi, five flavors, meridian entry, upbearing, downbearing, floating, sinking, toxin, etc."@en
    
    SubClassOf: 
        生理现象与过程
    
    
Class: 听气息

    Annotations: 
        rdfs:label "听气息"@zh,
        rdfs:label "Listening Sounds of Breathing"@zh
    
    SubClassOf: 
        闻诊
    
    
Class: 四气五味

    Annotations: 
        rdfs:label "Four qi and five flavors"@en,
        rdfs:label "四气五味"@zh,
        rdfs:comment "A collective term of four qi and five flavors. The four basic properties of medicinals, cold, hot, warmth, and coolness. The five tastes of medicinals, pungency, sweetness, sourness, bitterness, and saltiness, representing the basic actions of the medicinals."@en
    
    SubClassOf: 
        药性
    
    
Class: 治法

    Annotations: 
        rdfs:label "therapy"@en,
        rdfs:label "治法"@zh,
        rdfs:comment "Therapy, or treatment, is the attempted remediation of a health problem. Any specific intervention derived from a principle of treatment, e.g. diaphoresis, emesis, purgation, mediation, warming, clearing, tonification and resolution."@en
    
    SubClassOf: 
        中医治疗
    
    
Class: 疾病

    Annotations: 
        rdfs:comment "Study of disease process through basic theory of TCM."@en,
        rdfs:label "Disease"@en,
        rdfs:label "疾病"@zh
    
    SubClassOf: 
        病因病机疾病
    
    
Class: 现象与过程

    Annotations: 
        rdfs:label "现象与过程"@zh,
        rdfs:label "Phenomenon and process"@en,
        rdfs:label "A process or state which occurs naturally or as a result of an activity. (UMLS)"@en
    
    SubClassOf: 
        事件
    
    
Class: 功效

    Annotations: 
        rdfs:comment "Refers to the effect that Chinese medicinal produced on the body."@en,
        rdfs:label "The function of Chinese medicinal"@en,
        rdfs:label "功效"@zh
    
    SubClassOf: 
        中药属性和功能
    
    
Class: 脏

    Annotations: 
        rdfs:label "Viscus"@zh,
        rdfs:label "脏"@zh
    
    SubClassOf: 
        脏腑
    
    
Class: 切诊

    Annotations: 
        rdfs:label "切诊"@zh,
        rdfs:label "palpation"@en
    
    SubClassOf: 
        诊法
    
    
Class: 中医文献

    Annotations: 
        rdfs:comment "The body of written works (e.g., books, magazines) on the subject of traditional Chinese medicine."@en,
        rdfs:label "中医文献"@zh,
        rdfs:label "Traditional Chinese medicine literature"@en
    
    SubClassOf: 
        概念实体
    
    
Class: 中医药学科

    Annotations: 
        rdfs:comment "A subject that originated in China evolved a unique theoretical system, which is based on the Chinese people’s long-term medical practice."@en,
        rdfs:label "Traditional Chinese medicine subject"@en,
        rdfs:label "中医学科"@zh
    
    SubClassOf: 
        概念实体
    
    
Class: 形体关窍

    Annotations: 
        rdfs:comment "A collective term for skin, vessels, flesh, sinews, bones and the external opening of sense organs."@en,
        rdfs:label "Body constituent and orifice of sense organ"@en,
        rdfs:label "形体关窍"@zh
    
    SubClassOf: 
        中医人体基础
    
    
Class: 经络

    Annotations: 
        rdfs:comment "A system of conduits through which qi and blood circulate, connecting the bowels, viscera, extremities, superficial organs and tissues, making the body an organic whole, the same as channels and networks; meridians or channels, in short."@en,
        rdfs:comment "Meridian and collateral"@en,
        rdfs:comment "经络"@zh
    
    SubClassOf: 
        功能性人体系统
    
    
Class: 有机体

    Annotations: 
        rdfs:label "有机体"@zh,
        rdfs:label "Organism"@en
    
    SubClassOf: 
        物理对象
    
    
Class: 中医各家

    Annotations: 
        rdfs:label "Traditional Chinese Medicine Schools"@en,
        rdfs:label "中医各家"@zh,
        rdfs:comment "The prolonged history of traditional Chinese medicine has witnessed a plurality of famous figures, who not only inherited theories and experiences from their antecessors, but also formed their own opinions and doctrines.
The inheritance of academic tradition, achieved through apprenticeship training, in addition to the creativity of famous figures recognized for their outstanding works, gave rise to the different schools of traditional Chinese medicine.
"@en
    
    SubClassOf: 
        各家学说
    
    
Class: 诊法

    Annotations: 
        rdfs:comment "The basic method of collecting data to determine the disease condition."@en,
        rdfs:label "诊法"@zh,
        rdfs:label "Diagnostic method"@en
    
    SubClassOf: 
        中医诊断
    
    
Class: 病因病机疾病

    Annotations: 
        rdfs:label "Etiology, pathogenesis and disease"@en,
        rdfs:comment "Study of the etiology, development and mechanism of disease according to TCM theory."@en,
        rdfs:label "病因病机疾病"@zh
    
    SubClassOf: 
        现象与过程
    
    
Class: 按摩

    Annotations: 
        rdfs:label "按摩"@zh,
        rdfs:label "Massage"@en,
        rdfs:label "Rubbing, kneading, or percussion of the soft tissues and joints of the body with the hands, usually performed by one person on another, esp. to relieve tension or pain."@en
    
    SubClassOf: 
        治法
    
    
Class: 气功疗法

    Annotations: 
        rdfs:comment "Qigong is a therapeutic method used to prevent and cure disease by means of bringing the subjective initiative of the patient into full play."@en,
        rdfs:label "Qigong therapy"@en,
        rdfs:label "气功疗法"@zh
    
    SubClassOf: 
        治法
    
    
Class: 概念实体

    Annotations: 
        rdfs:label "概念实体"@zh,
        rdfs:comment "A broad type for grouping abstract entities or concepts."@en,
        rdfs:label "Conceptual entity"@en
    
    SubClassOf: 
        实体
    
    
Class: 中医心理

    Annotations: 
        rdfs:comment "Study of human psychological state according to TCM Theory."@en,
        rdfs:label "Traditional Chinese medicine psychology"@en,
        rdfs:label "中医心理"@zh
    
    SubClassOf: 
        生理现象与过程
    
    
Class: 辨证

    Annotations: 
        rdfs:label "辨证"@zh,
        rdfs:label "Syndrome differentiation"@en,
        rdfs:comment "The process of overall analysis of clinical data to determine the location, cause and nature of a patient’s disease and achieving a diagnosis of a pattern/syndrome, also called pattern differentiation."@en
    
    SubClassOf: 
        中医诊断
    
    
Class: 人体基本物质

    Annotations: 
        rdfs:comment "Basic substance in the human body"@en,
        rdfs:comment "人体基本物质"@zh
    
    SubClassOf: 
        中医人体基础
    
    
Class: 归经

    Annotations: 
        rdfs:label "归经"@zh,
        rdfs:comment "Orientation of the medicinal action according to the meridian/channel on which the therapeutic action is manifested, also called meridian tropism."@en,
        rdfs:label "Meridian entry"@en
    
    SubClassOf: 
        药性
    
    
Class: 听声音

    Annotations: 
        rdfs:label "听声音"@zh,
        rdfs:label "listening examination"@en
    
    SubClassOf: 
        闻诊
    
    
Class: 中医相关学科

    Annotations: 
        rdfs:label "Related subjects of traditional Chinese medicine"@en,
        rdfs:label "中医相关学科"@zh,
        rdfs:comment "Referring to a subject that is connected to Traditional Chinese Medicine."@en
    
    SubClassOf: 
        概念实体
    
    
Class: 各家学说

    Annotations: 
        rdfs:label "各家学说"@zh,
        rdfs:label "Theories of schools of traditional Chinese medicine"@en,
        rdfs:comment "Refers to a TCM theory that is from various factions."@en
    
    SubClassOf: 
        中医理论
    
    
Class: 中医治疗

    Annotations: 
        rdfs:label "Traditional Chinese medicine treatment"@en,
        rdfs:label "中医治疗"@zh,
        rdfs:comment "Treat the disease with the idea and method of syndrome differentiation and treatment."@en
    
    SubClassOf: 
        活动
    
    
Class: 闻气味

    Annotations: 
        rdfs:label "闻气味"@zh,
        rdfs:label "smelling examination"@en
    
    SubClassOf: 
        闻诊
    
    
Class: 中药疗法

    Annotations: 
        rdfs:comment "Under the guidance of the basic TCM theory, prescribe Chinese medicinal to treat the disease."@en,
        rdfs:label "Chinese medicinal therapy"@en,
        rdfs:label "中药疗法"@zh
    
    SubClassOf: 
        治法
    
    
Class: 动物

    Annotations: 
        rdfs:label "Animal"@en,
        rdfs:label "动物"@zh
    
    SubClassOf: 
        有机体
    
    
Class: Constitution

    Annotations: 
        rdfs:label "Constitution"@en,
        rdfs:comment "The characteristics of an individual, including structural and functional characteristics, temperament, adaptability to environmental changes and susceptibility to disease. It is relatively stable, being in part, genetically determined and in part, acquired."@en,
        rdfs:label "体质"@zh
    
    SubClassOf: 
        中医人体基础
    
    
Class: 药用物质

    Annotations: 
        rdfs:comment "用于诊断, 治愈, 移除, 治疗, 或预防疾病的物质."@zh,
        rdfs:label "Medicinal substance"@en,
        rdfs:comment "A substance intended for use in the diagnosis, cure, mitigation, treatment, or prevention of disease. This includes substances that occur naturally in the body and are administered therapeutically."@en,
        rdfs:label "药用物质"@zh
    
    SubClassOf: 
        物理对象
    
    
Class: 中医团体

    Annotations: 
        rdfs:label "A social group organized for some end or tasks related to health care, education, and scientific research in traditional Chinese medicine."@zh,
        rdfs:label "Traditional Chinese medicine organization"@en,
        rdfs:label "中医团体"@zh
    
    SubClassOf: 
        团体
    
    
Class: owl:Thing

    
Class: 腧穴

    Annotations: 
        rdfs:label "腧穴"@zh,
        rdfs:label "Acupuncture point"@en,
        rdfs:comment "The point where a needle is inserted and manipulated in acupuncture therapy."@en
    
    SubClassOf: 
        功能性人体系统
    
    
Class: 治则

    Annotations: 
        rdfs:comment "A general rule that should be followed in treating disease."@en,
        rdfs:label "Therapeutic principle"@en,
        rdfs:label "治则"@zh
    
    SubClassOf: 
        中医治疗
    
    
Class: 五脏

    Annotations: 
        rdfs:label "five viscera"@en,
        rdfs:label "五脏"@zh
    
    EquivalentTo: 
        {心 , 肝 , 肺 , 肾 , 脾}
    
    SubClassOf: 
        脏
    
    
Class: 津液

    Annotations: 
        rdfs:label "Liquid and humor"@en,
        rdfs:label "津液"@zh,
        rdfs:comment "A general term for all kinds of normal liquid in the body, except the blood, also known as body liquids."@en
    
    SubClassOf: 
        人体基本物质
    
    
Class: 医家

    Annotations: 
        rdfs:label "The people who dedicated their lives to the development of (traditional Chinese) medicine from ancient times , particularly the ancestors who are symbolized as Huangdi and Shennong."@en,
        rdfs:label "医家"@zh,
        rdfs:label "Medical specialist"@en
    
    SubClassOf: 
        各家学说
    
    
Class: 生理现象与过程

    Annotations: 
        rdfs:label "Phenomena or process that organism itself have or due to some activity."@en,
        rdfs:label "生理现象与过程"@zh,
        rdfs:label "Physiology phenomenon or process"@en
    
    SubClassOf: 
        现象与过程
    
    
Class: 证侯

    Annotations: 
        rdfs:label "Syndrome"@en,
        rdfs:comment "Summarization of the cause, nature and location of the pathological change at a certain stages of disease."@en,
        rdfs:label "证候"@zh,
        rdfs:label "pattern"@en,
        rdfs:comment "证候是中医对人体病变的分类体系."@zh
    
    SubClassOf: 
        病因病机疾病
    
    
Class: 物质

    Annotations: 
        rdfs:label "Substance"@en,
        rdfs:label "物质"@zh
    
    SubClassOf: 
        物理对象
    
    
Class: 脏腑

    Annotations: 
        rdfs:comment "A collective term for internal organs, also called zang-organs and fu-organs."@en,
        rdfs:label "脏腑"@zh,
        rdfs:label "Viscera & Bowel"@en
    
    SubClassOf: 
        功能性人体系统
    
    
Class: 中华传统哲学

    Annotations: 
        rdfs:comment "Philosophical thought that was developed by ancient Chinese, through the generalization and summarization of their natural and social knowledge."@en,
        rdfs:label "中华传统哲学"@zh,
        rdfs:label "Traditional Chinese philosophy"@en
    
    SubClassOf: 
        中医相关学科
    
    
Class: 中医相关自然物理学科

    Annotations: 
        rdfs:comment "A subject that involves the study of natural phenomena or physical phenomena related TCM."@en,
        rdfs:label "Related nature physics subjects of traditional Chinese medicine"@en,
        rdfs:label "中医相关自然物理学科"@zh
    
    SubClassOf: 
        中医相关学科
    
    
Class: 望诊

    Annotations: 
        rdfs:label "Inspection"@zh,
        rdfs:label "望诊"@zh
    
    SubClassOf: 
        诊法
    
    
Class: 中药属性和功能

    Annotations: 
        rdfs:label "Property and function of Chinese medicinal"@en,
        rdfs:label "中药属性和功能"@zh,
        rdfs:comment "Refer to the property, flavor, meridian entry, upbearing, downbearing, floating and sinking, toxin, and function of traditional Chinese drugs."@en
    
    SubClassOf: 
        现象与过程
    
    
Class: 腑

    Annotations: 
        rdfs:label "腑"@zh,
        rdfs:label "bowel"@en
    
    SubClassOf: 
        脏腑
    
    
Class: 七情

    Annotations: 
        rdfs:label "七情"@zh,
        rdfs:label "Seven emotions"@en,
        rdfs:label "A collective term for joy, anger, thought, anxiety, sorrow, fear and fright, taken as endogenous factors causing diseases if in excess."@en
    
    SubClassOf: 
        中医心理
    
    
Class: 方剂

    Annotations: 
        rdfs:comment "Formula refers to herbal formula in TCM domain, which is prescriptions as mixtures of multiple herbs."@en,
        rdfs:label "Formula"@en,
        rdfs:comment "方剂指由若干中草药混合而成的处方."@zh,
        rdfs:label "方剂"@zh
    
    EquivalentTo: 
        药用物质
         and (包含 some 药用物质)
         and (治疗 some 证侯)
    
    SubClassOf: 
        药用物质
    
    
Class: 针灸疗法

    Annotations: 
        rdfs:comment "Treatment of disease by inserting needles along specific pathways or meridians. The placement varies with the disease being treated. It is sometimes used in conjunction with heat, moxibustion, acupressure, or electric stimulation."@en,
        rdfs:label "Acupuncture therapy"@en,
        rdfs:label "针灸疗法"@zh
    
    SubClassOf: 
        治法
    
    
Class: 神

    Annotations: 
        rdfs:label "Mind"@en,
        rdfs:label "Mental activities, referring to mind, consciousness, thinking and feeling."@en,
        rdfs:label "神"@zh
    
    SubClassOf: 
        中医心理
    
    
Class: 阴阳理论

    Annotations: 
        rdfs:label "阴阳理论"@zh,
        rdfs:label "Yin-yang theory"@en,
        rdfs:comment "An ancient Chinese philosophical concept, dealing with two opposite aspects of matters in nature which are interrelated with each other. Its principle is widely applied to traditional Chinese medicine."@en
    
    SubClassOf: 
        中医理论
    
    
Class: 毒性

    Annotations: 
        rdfs:comment "Any virulent pathogen that causes a fulminating disease."@en,
        rdfs:label "毒性"@zh,
        rdfs:label "Toxin"@en
    
    SubClassOf: 
        药性
    
    
Class: 五行理论

    Annotations: 
        rdfs:label "五行理论"@zh,
        rdfs:comment "One of the philosophical theories of medical practice in ancient China, concerning the composition and evolution of the physical universe, epitomized by the nature and the inhibition-generation relationships of the five phases, wood, fire, earth, metal and water, serving as the guiding ideology and methodology of physiology, pathology, clinical diagnosis and treatment, also known as five elements theory."@en,
        rdfs:label "Five phase theory"@en
    
    SubClassOf: 
        中医理论
    
    
Class: 病因病机

    Annotations: 
        rdfs:comment "Study of the cause, development, and mechanism of disease according to the basic theory of TCM."@en,
        rdfs:label "病因病机"@zh,
        rdfs:label "Etiology and pathogenesis"@en
    
    SubClassOf: 
        病因病机疾病
    
    
Class: 配伍

    Annotations: 
        rdfs:label "配伍"@zh,
        rdfs:label "Chinese medicinal combination"@en,
        rdfs:comment "Use various medicinals jointly in a formula or prescription for producing the desired therapeutic effect and reducing toxic or side effects."@en
    
    SubClassOf: 
        功效
    
    
Class: 闻诊

    Annotations: 
        rdfs:label "listening and smelling examination"@en,
        rdfs:label "闻诊"@zh
    
    SubClassOf: 
        诊法
    
    
Class: 血

    Annotations: 
        rdfs:comment "血"@zh,
        rdfs:comment "Blood"@en,
        rdfs:comment "The red fluid circulating through the blood vessels, and nourishing and moistening the whole body."@en
    
    SubClassOf: 
        人体基本物质
    
    
Class: 四诊

    Annotations: 
        rdfs:label "four examinations"@en,
        rdfs:label "四诊"@zh
    
    EquivalentTo: 
        切诊
         or 望诊
         or 问诊
         or 闻诊
    
    SubClassOf: 
        诊法
    
    
Class: 中医生理功能

    Annotations: 
        rdfs:comment "Study of human physiological state according to TCM Theory."@en,
        rdfs:label "中医生理功能"@zh,
        rdfs:label "Traditional Chinese medicine physiological function"@en
    
    SubClassOf: 
        生理现象与过程
    
    
Class: 中药化学成分

    Annotations: 
        rdfs:label "中药化学成分"@zh,
        rdfs:comment "Molecular components that are extracted from Chinese medicinal after extraction, separation, identification, structure determination."@zh,
        rdfs:label "Chemical constituent of Chinese medicine"@en
    
    EquivalentTo: 
        化学物质
         and 药用物质
    
    SubClassOf: 
        药用物质
    
    
Class: 活动

    Annotations: 
        rdfs:label "活动"@zh,
        rdfs:label "Activity"@en,
        rdfs:label "An operation or series of operations that an organism or machine carries out or participates in."@en
    
    SubClassOf: 
        事件
    
    
Class: 饮食疗法

    Annotations: 
        rdfs:label "Diet therapy"@en,
        rdfs:label "饮食疗法"@zh,
        rdfs:comment "Also known as the food therapy. It is a way that will regulate the body and treat disease according to the different nature of food flavors and acting on different organs. Use nutritious food or medicinal food products to reinforce the healthy qi and strong physique."@en
    
    SubClassOf: 
        治法
    
    
Class: 问诊

    Annotations: 
        rdfs:label "问诊"@zh,
        rdfs:label "Inquiry"@zh
    
    SubClassOf: 
        诊法
    
    
Class: 中医诊断

    Annotations: 
        rdfs:label "中医诊断"@en,
        rdfs:comment "Determination of the nature of a diseased condition; identification of a disease by careful investigation of its symptoms and history; also, the opinion (formally stated) resulting from such investigation."@en,
        rdfs:label "Traditional Chinese diagnostics"@en
    
    SubClassOf: 
        活动
    
    
Class: 药用矿物

    Annotations: 
        rdfs:label "药用矿物"@zh,
        rdfs:comment "A naturally occurring, homogeneous inorganic solid substance having a definite chemical composition, and have health function or can be used to prevent and treat the disease."@en,
        rdfs:label "Medicinal mineral"@en
    
    SubClassOf: 
        药用动物植物矿物
    
    
Class: 中药

    Annotations: 
        rdfs:label "中药"@zh,
        rdfs:label "Chinese medicinal"@en,
        rdfs:comment "Usually referring to those medicinal substances recorded in Chinese materia medica."@en
    
    EquivalentTo: 
        药用物质
         and (治疗 some 病因病机疾病)
    
    SubClassOf: 
        药用物质
    
    
Class: 药用植物

    Annotations: 
        rdfs:comment "Generally refers to those plants that have health function or can be used to prevent and treat the disease."@en,
        rdfs:label "Medicinal plant"@en,
        rdfs:label "药用植物"@zh
    
    SubClassOf: 
        药用动物植物矿物
    
    
Individual: 肾虚证

    Annotations: 
        rdfs:label "Kideny Deficiency"@en,
        rdfs:label "kidney deficiency syndrome"@en,
        rdfs:label "肾虚证"@zh
    
    Types: 
        证侯
    
    Facts:  
     的病位是  肾
    
    
Individual: 石杉碱甲

    Annotations: 
        rdfs:isDefinedBy <Http://www.catcm.ac.cn/doc/64010>,
        rdfs:label "石杉碱甲"@zh,
        rdfs:label "Huperzine A"@en,
        rdfs:seeAlso <Http://www.catcm.ac.cn/doc/64010>,
        rdfs:comment "Huperzine A is a naturally occurring sesquiterpene alkaloid found in the extracts of the firmoss Huperzia serrata."@en
    
    Types: 
        化学物质,
        药用物质
    
    Facts:  
     治疗  记忆减退,
     治疗  阿尔茨海默症,
     治疗  肾阳证
    
    
Individual: 白术

    Annotations: 
        rdfs:label "白术"@zh,
        rdfs:label "Atractylodes"@en
    
    Types: 
        中药
    
    
Individual: 肾阳证

    Annotations: 
        rdfs:label "kidney yang syndrome"@en,
        rdfs:label "肾阳证"@zh
    
    Types: 
        证侯
    
    
Individual: 咸

    Annotations: 
        rdfs:label "咸"@zh,
        rdfs:label "Salty"@en
    
    Types: 
        四气五味
    
    
Individual: 阳证

    Annotations: 
        rdfs:label "阳证"@zh,
        rdfs:label "yang syndrome"@zh
    
    Types: 
        证侯
    
    
Individual: 脾

    Annotations: 
        rdfs:label "脾"@zh,
        rdfs:label "Spleen"@en
    
    Types: 
        脏
    
    
Individual: 虚证

    Annotations: 
        rdfs:label "虚证"@zh,
        rdfs:label "Deficiency"@en
    
    Types: 
        证侯
    
    Facts:  
     传递性下位概念  肾虚证,
     传递性下位概念  肾阳证,
     传递性下位概念  阳证
    
    
Individual: 人参

    Annotations: 
        rdfs:label "Ginseng"@en,
        rdfs:label "人参"@zh
    
    Types: 
        中药
    
    Facts:  
     治疗  虚证,
     有药味  甜,
     有药味  苦
    
    
Individual: 水

    Annotations: 
        rdfs:comment "水"@zh,
        rdfs:label "水"@zh,
        rdfs:label "Water"@en
    
    Types: 
        五行
    
    Facts:  
     滋养  木
    
    
Individual: 肾阳虚证

    Annotations: 
        rdfs:label "肾阳虚证"@zh,
        rdfs:label "Kideny Yang Deficiency"@en
    
    Types: 
        证侯
    
    Facts:  
     传递性上位概念  虚证,
     相关关系链  记忆减退,
     相关关系链  怀孕,
     传递性上位概念  肾虚证,
     传递性上位概念  阳证,
     相关关系链  阿尔茨海默症
    
    
Individual: 肝

    Annotations: 
        rdfs:label "肝"@zh,
        rdfs:label "Liver"@en
    
    Types: 
        脏
    
    
Individual: 甜

    Annotations: 
        rdfs:label "甜"@zh,
        rdfs:label "Sweet"@en
    
    Types: 
        四气五味
    
    
Individual: 记忆减退

    Annotations: 
        rdfs:label "记忆减退"@zh,
        rdfs:label "Memory Loss"@en
    
    Types: 
        症状体征
    
    Facts:  
     相关关系链  肾阳证
    
    
Individual: 辛

    Annotations: 
        rdfs:label "Pungent"@en,
        rdfs:label "辛"@zh
    
    Types: 
        四气五味
    
    
Individual: 木

    Annotations: 
        rdfs:label "Wood"@en,
        rdfs:comment "木"@zh,
        rdfs:label "木"@zh
    
    Types: 
        五行
    
    
Individual: 怀孕

    Annotations: 
        rdfs:label "怀孕"@zh,
        rdfs:label "pregnancy"@en
    
    Types: 
        临床状况
    
    
Individual: 苦

    Annotations: 
        rdfs:label "苦"@zh,
        rdfs:label "Bitter"@en
    
    Types: 
        四气五味
    
    
Individual: 四君子汤

    Annotations: 
        rdfs:label "four gentlemen decoction"@en,
        rdfs:label "四君子汤"@zh,
        rdfs:label "Four gentlemen decoction"@en
    
    Types: 
        方剂,
        药用物质
    
    Facts:  
     包含  人参,
     治疗  肾阳证,
     君药  人参,
     佐药  茯苓,
     使药  甘草,
     治疗  肾虚证,
     臣药  白术
    
    
Individual: 甘草

    Annotations: 
        rdfs:label "Glycyrrhizae"@en,
        rdfs:label "甘草"@zh
    
    Types: 
        中药
    
    
Individual: 肺

    Annotations: 
        rdfs:label "Lung"@en,
        rdfs:label "肺"@zh
    
    Types: 
        脏
    
    
Individual: 千层塔

    Annotations: 
        rdfs:label "千层塔"@zh,
        rdfs:label "Huperzia serrata"@en
    
    Types: 
        中药
    
    Facts:  
     包含化学物质  石杉碱甲
    
    
Individual: 肾

    Annotations: 
        rdfs:label "Kidney"@en,
        rdfs:label "肾"@zh
    
    Types: 
        脏
    
    
Individual: 心

    Annotations: 
        rdfs:label "心"@zh,
        rdfs:label "Heart"@en
    
    Types: 
        脏
    
    
Individual: 茯苓

    Annotations: 
        rdfs:label "Fu Ling"@en,
        rdfs:label "茯苓"@zh
    
    Types: 
        中药
    
    
Individual: 阳虚证

    Annotations: 
        rdfs:label "阳虚证"@zh,
        rdfs:label "Yang Deficiency"@en
    
    Types: 
        证侯
    
    
Individual: 阿尔茨海默症

    Annotations: 
        rdfs:comment "以渐进性痴呆为特征的人类退化性紊乱."@zh,
        rdfs:comment "A human degenerative disorder characterized by progressive dementia."@en,
        rdfs:label "阿尔茨海默症"@zh,
        rdfs:label "Alzheimer's Disease"@en
    
    Types: 
        疾病
    
    
Individual: 酸

    Annotations: 
        rdfs:label "酸"@zh,
        rdfs:label "Sour"@en
    
    Types: 
        四气五味
    
    
